merged hint_list with core

SetSpecs.v
@@ -25,13 +25,13 @@ Require Export Lists.List.
 
 Set Implicit Arguments.
 
-Hint Resolve in_eq in_cons in_inv in_nil in_dec: hint_list.
+Hint Resolve in_eq in_cons in_inv in_nil in_dec: core.
 
 Section BasicListFacts.
   Variable A:Type.
   Lemma in_inv1 : forall (a b:A) (l:list A), In b (a :: l) -> b = a \/ In b l.
   Proof. { intros  a b l H. cut (a=b \/ In b l).
-       Focus 2. auto with hint_list. intros H1; destruct H1 as [H1 | H2].
+       Focus 2. auto.  intros H1; destruct H1 as [H1 | H2].
        left; symmetry; auto. right;auto. } Qed.
   Lemma in_inv2: forall (x a:A) (l:list A), In x (a::l)-> x <> a -> In x l.
   Proof.  { intros x a l H. cut (x=a \/ In x l). intro H1;destruct H1 as [Hl1|Hr1].
@@ -39,7 +39,7 @@ Section BasicListFacts.
   Lemma in_inv3: forall (x a:A) (l:list A), In x (a::l)-> ~ In x l -> x = a.
     Proof.  { intros x a l H. cut (x=a \/ In x l). intro H1;destruct H1 as [Hl1|Hr1].
           intro;auto. intro;contradiction.  eapply in_inv1;auto. } Qed.
-  Hint Resolve in_inv1 in_inv2 in_inv3 : hint_list.
+  Hint Resolve in_inv1 in_inv2 in_inv3 : core.
   (*---------Some facts about NoDup on a list --------------------------------*)
   Lemma nodup_intro (a:A)(l: list A): ~ In a l -> NoDup l -> NoDup (a::l).
     Proof.  intros H1 H2; eapply NoDup_cons_iff;tauto.  Qed. 
@@ -48,19 +48,19 @@ Section BasicListFacts.
   Lemma nodup_elim2 (a:A)(l: list A): NoDup (a::l) -> ~ In a l.
     Proof. intro H. eapply NoDup_cons_iff; eauto. Qed. 
   
-  Hint Immediate nodup_elim1  nodup_elim2  nodup_intro : hint_list.
+  Hint Immediate nodup_elim1  nodup_elim2  nodup_intro : core.
   End BasicListFacts.
-Hint Resolve in_inv1 in_inv2 in_inv3: hint_list.
-Hint Immediate nodup_elim1  nodup_elim2  nodup_intro : hint_list.
-Hint Immediate nodup_elim1  nodup_elim2  nodup_intro : hint_nodup.
+Hint Resolve in_inv1 in_inv2 in_inv3: core.
+Hint Immediate nodup_elim1  nodup_elim2  nodup_intro : core.
 
 
 
 Section SetSpec.
   Variable A:Type.
   Definition Empty (s:list A):Prop := forall a : A, ~ In a s.
-  Definition Equal (s s': list A) := forall a : A, In a s <-> In a s'.
+  (* Definition Equal (s s': list A) := forall a : A, In a s <-> In a s'. *)
   Definition Subset (s s': list A) := forall a : A, In a s -> In a s'.
+  Definition Equal (s s': list A):= Subset s s' /\ Subset s' s.
   Print Forall.
   (* Inductive Forall (A : Type) (P : A -> Prop) : list A -> Prop := 
      | Forall_nil : Forall P nil 
@@ -89,27 +89,45 @@ Section BasicSetFacts.
 
   (*-----------------------Subset (spec) and its properties ------------------------*)
   
-  Lemma Subset_elim1 (a:A) (s s':list A): Subset (a:: s) s'-> In a s' /\ Subset s s'.
-  Proof. { unfold Subset. intro H. split. apply H. auto with hint_list. intros a1 H1.
-           apply H. auto with hint_list. } Qed.
+  Lemma Subset_elim1 (a:A) (s s':list A): Subset (a:: s) s'-> In a s'.
+  Proof. { unfold Subset. intro H. apply H. auto. } Qed.
+   Lemma Subset_elim2 (a:A) (s s':list A): Subset (a:: s) s'->  Subset s s'.
+  Proof. { unfold Subset. intro H.  intros a1 H1.
+           apply H. auto. } Qed.
   Lemma self_incl (l:list A): l [<=] l.
   Proof. unfold Subset; tauto.  Qed. 
-  Hint Resolve self_incl: hint_set.
+  Hint Resolve self_incl: core.
 
   Lemma Subset_nil (l: list A): nil [<=] l.
-    Proof. unfold "[<=]"; simpl; intros; contradiction. Qed.
+  Proof. unfold "[<=]"; simpl; intros; contradiction. Qed.
 
+  Lemma Subset_trans (l1 l2 l3: list A): l1 [<=] l2 -> l2 [<=] l3 -> l1 [<=] l3.
+  Proof. intros H H1 x Hx1. eauto. Qed. 
+   
+Hint Extern 0 (?x [<=] ?z)  =>
+match goal with
+| H: (x [<=] ?y) |- _ => apply (@Subset_trans  x y z)
+| H: (?y [<=] z) |- _ => apply (@Subset_trans  x y z)                                   
+end.
   
   (* ---------------------- Equal (spec) and their properties--------------------*)
   Lemma Eq_refl (s: list A):  s [=] s.
-  Proof.  unfold Equal. tauto.  Qed. 
+  Proof.  unfold Equal. split;auto using self_incl.  Qed. 
   Lemma Eq_sym (s s':list A): s [=] s' -> s' [=] s.
-  Proof. unfold Equal. unfold iff. intros H a. specialize (H a). tauto. Qed. 
+  Proof. unfold Equal.  tauto. Qed. 
   Lemma Eq_trans1 ( x y z : list A) : x [=] y -> y [=] z -> x [=] z.
-  Proof. { unfold Equal. unfold iff. intros H H1 a.
-         specialize (H1 a). specialize (H a). tauto. } Qed. 
+  Proof. { unfold Equal.  intros H H1. destruct H as [H0 H]; destruct H1 as [H1a H1].
+           split; auto. } Qed.
+
+ Hint Extern 0 (?x [=] ?z)  =>
+match goal with
+| H: (x [=] ?y) |- _ => apply (@Eq_trans1  x y z)
+| H: (?y [=] z) |- _ => apply (@Eq_trans1  x y z)                                   
+end.
+
+
   Lemma Equal_intro (s s': list A): s [<=] s' -> s' [<=] s -> s [=] s'.
-  Proof. unfold_spec. intros H H1 a; unfold iff. auto. Qed.
+  Proof. unfold "[=]".  tauto. Qed.
   Lemma Equal_intro1 (s s': list A): s = s' -> Equal s s'.
   Proof. intro; subst s; apply Eq_refl; auto. Qed.
   Lemma Equal_elim ( s s': list A): s [=] s' ->  s [<=] s' /\ s' [<=] s.
@@ -117,11 +135,28 @@ Section BasicSetFacts.
  
 End BasicSetFacts.
 
+
+
  Notation "s [=] t" := (Equal s t) (at level 70, no associativity).
  Notation "s [<=] t" := (Subset s t) (at level 70, no associativity).
  Notation "| s |":= (length s) (at level 70, no associativity).
 
-Hint Immediate Eq_refl Eq_sym Eq_trans1 Equal_elim Equal_intro Equal_intro1: hint_list.
-Hint Immediate Subset_elim1 Subset_nil : hint_list.
-Hint Resolve  self_incl Eq_trans1: hint_list.
+   
+Hint Extern 0 (?x [<=] ?z)  =>
+match goal with
+| H: (x [<=] ?y) |- _ => apply (@Subset_trans _ x y z)
+| H: (?y [<=] z) |- _ => apply (@Subset_trans _ x y z)                                   
+end.
+
+Hint Extern 0 (?x [=] ?z)  =>
+match goal with
+| H: (x [=] ?y) |- _ => apply (@Eq_trans1 _ x y z)
+| H: (?y [=] z) |- _ => apply (@Eq_trans1 _ x y z)                                   
+end.
+
+
+Hint Immediate Eq_refl Eq_sym Equal_elim Equal_intro Equal_intro1: core.
+Hint Immediate Subset_elim1 Subset_elim2 Subset_nil : core.
+Hint Resolve  self_incl: core.
+
 
